examples/low-level/crypto/Crypto.AEAD.Invariant.fst
@@ -29,10 +29,52 @@ module PRF = Crypto.Symmetric.PRF
 let min (a:u32) (b:u32) = if a <=^ b then a else b
 let minNat (a:nat) (b:nat) : nat = if a <= b then a else b
 
-type region = rgn:HH.rid {HS.is_eternal_region rgn}
+type eternal_region = rgn:HH.rid {HS.is_eternal_region rgn}
 
-let ctr x = PRF.(x.ctr)
+let prf_table (r:rgn) (i:id) = Seq.seq (PRF.entry r i)
 
+(*** COUNTERS AND LENGTHS ***)
+(* The ctr value associated with the first otp block *)
+let otp_offset (i:id) = ctr_0 i +^ 1ul
+
+let maxplain (i:id) = pow2 14 // for instance
+
+let num_blocks_for_len (i:id) (l:nat) : Tot nat =
+  let bl = v (Cipher.( blocklen (cipherAlg_of_id i))) in
+  (l + bl - 1) / bl
+
+(** safelen: The length of the plaintext is not too large **)
+let safelen (i:id)
+	    (remaining_len:nat)  //the length of plaintext left to be encrypted;
+	    (next_block_index:UInt32.t) //the counter for encrypting the next block of plaintext
+  =
+  let open FStar.Mul in
+  PRF.ctr_0 i <^ next_block_index &&                  //next_block_index is strictly greater than the mac domain position
+  next_block_index <=^ PRF.maxCtr i &&               //and less then the max counter
+  (let block_length = v (Cipher.(blocklen (cipherAlg_of_id i))) in
+   let len_all_blocks_so_far = v (next_block_index -^ PRF.ctr_0 i -^ 1ul) * block_length in
+   let max_len_for_remaining_blocks = v (PRF.maxCtr i -^ next_block_index) * block_length in
+   remaining_len = 0 ||                               //no more text left to encrypt, or
+   (remaining_len + len_all_blocks_so_far <= maxplain i &&
+    remaining_len <= max_len_for_remaining_blocks))
+
+(** remaining_len_ok: 
+      Given a plaintext of length len, with remaining_len left to encrypt,
+      the current_block_index accurately characterizes the number of blocks 
+      already encrypted **)
+let remaining_len_ok (#i:id) (current_block_index:PRF.domain i) (len:u32) (remaining_len:u32) =
+  PRF.ctr_0 i <^ current_block_index.ctr &&
+  safelen i (v remaining_len) current_block_index.ctr &&
+  remaining_len <=^ len &&
+  len <> 0ul &&
+  safelen i (v len) (otp_offset i) &&
+  (let completed_len = v len - v remaining_len in
+   let n_blocks = v current_block_index.ctr - v (otp_offset i) in
+   if remaining_len = 0ul then
+      n_blocks = num_blocks_for_len i (v len)
+   else completed_len = FStar.Mul.(n_blocks * v (PRF.blocklen i)))
+
+(*** THE TYPE OF AEAD KEYS ***)
 noeq type aead_entry (i:id) =
   | AEADEntry:
       nonce:Cipher.iv (alg i) ->
@@ -42,15 +84,7 @@ noeq type aead_entry (i:id) =
       c:cipher i (Seq.length (as_bytes p)) ->
       aead_entry i
 
-let prf_table (r:rgn) (i:id) = Seq.seq (PRF.entry r i)
 let aead_entries i = Seq.seq (aead_entry i)
-
-noextract let is_aead_entry_nonce (#i:id) (n:Cipher.iv (alg i)) (e:aead_entry i) =
-  e.nonce = n
-
-noextract let find_aead_entry (#i:id) (n:Cipher.iv (alg i)) (entries:Seq.seq (aead_entry i))
-  : option (aead_entry i)
-  = SeqProperties.find_l (is_aead_entry_nonce n) entries
 
 noeq type aead_state (i:id) (rw:rw) =
   | AEADState:
@@ -66,43 +100,44 @@ noeq type aead_state (i:id) (rw:rw) =
       ak: CMA.akey prf.mac_rgn i (* static, optional authentication key *) ->
       aead_state i rw
 
+(*** MAIN STATEFUL INVARIANT ***)
+
+(** Some utilities for stating the invariant **)
+noextract let is_aead_entry_nonce (#i:id) (n:Cipher.iv (alg i)) (e:aead_entry i) =
+  e.nonce = n
+
+noextract let find_aead_entry (#i:id) (n:Cipher.iv (alg i)) (entries:Seq.seq (aead_entry i))
+  : option (aead_entry i)
+  = SeqProperties.find_l (is_aead_entry_nonce n) entries
+
 let fresh_nonce (#i:id) (#rw:rw) (n:Cipher.iv (alg i)) (aead_st:aead_state i rw) (h:mem) = 
   let entries = HS.sel h aead_st.log in
   None? (find_aead_entry n entries)
 
-let maxplain (i:id) = pow2 14 // for instance
+let num_blocks_for_entry (#i:id) (e:aead_entry i) : Tot nat =
+  let AEADEntry nonce ad l plain cipher_tagged = e in
+  num_blocks_for_len i l
 
-(* safelen: The length of the plaintext is not too large *)
-let safelen (i:id)
-	    (remaining_len:nat)  //the length of plaintext left to be encrypted;
-	    (next_block_index:UInt32.t) //the counter for encrypting the next block of plaintext
-  =
-  let open FStar.Mul in
-  PRF.ctr_0 i <^ next_block_index &&                  //next_block_index is strictly greater than the mac domain position
-  next_block_index <=^ PRF.maxCtr i &&               //and less then the max counter
-  (let block_length = v (Cipher.(blocklen (cipherAlg_of_id i))) in
-   let len_all_blocks_so_far = v (next_block_index -^ PRF.ctr_0 i -^ 1ul) * block_length in
-   let max_len_for_remaining_blocks = v (PRF.maxCtr i -^ next_block_index) * block_length in
-   remaining_len = 0 ||                               //no more text left to encrypt, or
-   (remaining_len + len_all_blocks_so_far <= maxplain i &&
-    remaining_len <= max_len_for_remaining_blocks))
+let encode_ad_cipher (i:id) (ad:adata) (l:plainLen{safelen i l (PRF.ctr_0 i +^ 1ul)}) (cipher:lbytes l) =
+  encode_both i (FStar.UInt32.uint_to_t (Seq.length ad)) ad (FStar.UInt32.uint_to_t l) cipher
 
-// Computes PRF table contents for countermode encryption of 'plain' to 'cipher' starting from 'x'.
+(** counterblocks:
+         A sequence of OTP entries for the PRF table
+	 corresponding to the fragmentation of the 
+	 plain and cipher into encrypted blocks, 
+	 starting from position x, until to_pos **)
 val counterblocks:
-  i:id {safeId i} ->
-  rgn:region ->  //the rgn is really superfluous,
-		//since it is only potentially relevant in the case of the mac,
-		//but that's always Seq.createEmpty here
-                //16-10-13 but still needed in the result type, right?
-  x:PRF.domain i{PRF.ctr_0 i <^ ctr x} ->
+  i:id{safeId i} ->
+  mac_rgn:eternal_region ->
+  x:PRF.domain i{PRF.ctr_0 i <^ PRF.(x.ctr)} ->
   l:nat ->
   from_pos:nat ->
-  to_pos:nat{from_pos <= to_pos /\ to_pos <= l /\ safelen i (to_pos - from_pos) (ctr x)} ->
+  to_pos:nat{from_pos <= to_pos /\ to_pos <= l /\ safelen i (to_pos - from_pos) PRF.(x.ctr)} ->
   plain:Crypto.Plain.plain i l ->
   cipher:lbytes l ->
-  Tot (prf_table rgn i) // each entry e {PRF(e.x.id = x.iv /\ e.x.ctr >= ctr x)}
+  Tot (prf_table mac_rgn i) // each entry e {PRF(e.x.id = x.iv /\ e.x.ctr >= ctr x)}
   (decreases (to_pos - from_pos))
-let rec counterblocks i rgn x l from_pos to_pos plain cipher =
+let rec counterblocks i mac_rgn x l from_pos to_pos plain cipher =
   let blockl = v (Cipher.(blocklen (cipherAlg_of_id i))) in
   let remaining = to_pos - from_pos in
   if remaining = 0 then
@@ -112,21 +147,14 @@ let rec counterblocks i rgn x l from_pos to_pos plain cipher =
     let l_32 = UInt32.uint_to_t l0 in
     let plain_hd = Crypto.Plain.slice plain from_pos (from_pos + l0) in
     let cipher_hd = Seq.slice cipher from_pos (from_pos + l0) in
-    let block = PRF.Entry x (PRF.OTP l_32 plain_hd cipher_hd) in
-    let blocks = counterblocks i rgn (PRF.incr i x) l (from_pos + l0) to_pos plain cipher in
+    //safeId i is needed here, to show that OTP is a suitable range
+    let block = PRF.Entry x (PRF.OTP l_32 plain_hd cipher_hd) in 
+    let blocks = counterblocks i mac_rgn (PRF.incr i x) l (from_pos + l0) to_pos plain cipher in
     SeqProperties.cons block blocks
 
-let num_blocks_for_len (i:id) (l:nat) : Tot nat =
-  let bl = v (Cipher.( blocklen (cipherAlg_of_id i))) in
-  (l + bl - 1) / bl
-
-let num_blocks_for_entry (#i:id) (e:aead_entry i) : Tot nat =
-  let AEADEntry nonce ad l plain cipher_tagged = e in
-  num_blocks_for_len i l
-
-let encode_ad_cipher (i:id) (ad:adata) (l:plainLen{safelen i l (PRF.ctr_0 i +^ 1ul)}) (cipher:lbytes l) =
-  encode_both i (FStar.UInt32.uint_to_t (Seq.length ad)) ad (FStar.UInt32.uint_to_t l) cipher
-
+(** mac_is_set prf_table iv: 
+        the mac entry in the prf_table, at location (iv, ctr_0 i)
+	is set to the suitable encoded ad + cipher, tag      **)
 #reset-options "--z3rlimit 100 --initial_fuel 0 --max_fuel 0 --initial_ifuel 0 --max_ifuel 0"
 let mac_is_set (#rgn:region) (#i:id)
 	       (prf_table:prf_table rgn i{safeId i}) //the entire prf table
@@ -137,7 +165,7 @@ let mac_is_set (#rgn:region) (#i:id)
 	       (tag:MAC.tag)
 	       (h:mem) : GTot Type0
   = let dom_0 = {iv=iv; ctr=PRF.ctr_0 i} in
-    //2. the mac entry for this nonce in the prf table contains a mac'd ad+cipher
+    //the mac entry for this nonce in the prf table contains a mac'd ad+cipher
     (match PRF.find_mac prf_table dom_0 with
      | None -> False
      | Some mac_range ->
@@ -150,6 +178,11 @@ let mac_is_set (#rgn:region) (#i:id)
 	 msg = encode_ad_cipher i ad l cipher /\
  	 tag = tag'))
 
+(** refines_one_entry:
+        Conceptually, read it as (prf_table `refines_one_entry` aead_entry)
+	It states that there are entries in the prf_table (order unspecified)
+	that contains the mac and otp entries corresponding to aead_entry
+**)
 let refines_one_entry (#rgn:region) (#i:id)
 		      (prf_table:prf_table rgn i) //the entire prf table
 		      (aead_entry:aead_entry i)   //a single aead_entry
@@ -171,13 +204,32 @@ let refines_one_entry (#rgn:region) (#i:id)
       otp_blocks `contains` prf_entry ==>
       PRF.find prf_table prf_entry.x == Some (prf_entry.range)))
 
+(** none_above x prf_table:
+	no entry in the prf_table at ({iv=x.iv; ctr=i}) for any i >= x.ctr **)
 let none_above (#r:region) (#i:id) (x:PRF.domain i) (prf_table:prf_table r i) =
     forall (y:PRF.domain i{y `PRF.above` x}). PRF.find prf_table y == None
 
-let all_above (#rgn:region) (#i:id) (s:prf_table rgn i) (x:PRF.domain i) =
+(** none_above_if_authId x prf_state h:
+        A stateful variant of none_above, using the full prf_table in h **)
+let none_above_if_authId (#i:id) (x:PRF.domain i) (st:PRF.state i) (h:mem) =
+  CMA.authId (i, x.iv) ==>
+    (let prf_table = HS.sel h (itable i st) in
+     none_above x prf_table)
+
+(** all_above x prf_blocks
+	every entry in the prf_blocks is above x  ({iv=x.iv; ctr=i}) for any i >= x.ctr
+
+	This is generally used for some sequence of prf entries,
+	not the full prf table
+**)
+let all_above (#rgn:region) (#i:id) (x:PRF.domain i) (s:prf_table rgn i) =
   (forall (e:PRF.entry rgn i).{:pattern (s `SeqProperties.contains` e)}
      s `SeqProperties.contains` e ==> e.x `PRF.above` x)
 
+(** unused_aead_iv_for_prf prf_table iv:
+	the iv is either fresh, i.e., doesn't appear anywhere in the prf_table
+	Or, it occurs there with an unused mac (e.g., decrypt allocated one early)
+ **)
 let unused_aead_iv_for_prf (#mac_rgn:region) (#i:id)
 			   (prf_table:prf_table mac_rgn i) //the entire prf table
   			   (iv:Cipher.iv (alg i))
@@ -188,28 +240,36 @@ let unused_aead_iv_for_prf (#mac_rgn:region) (#i:id)
      | None           -> True //and no MAC entry either
      | Some mac_range -> CMA.mac_is_unset (i, iv) mac_rgn mac_range h) //Or, a mac exists, but it's not yet used
 
-(** THE MAIN CLAUSE OF THE STATEFUL INVARIANT:
-    States consistency of the PRF table contents vs the AEAD entries
+(** refines prf_table aead_entries h:
+	THE MAIN CLAUSE OF THE STATEFUL INVARIANT:
+	In state h, prf_table refines aead_entries
  **)
 let refines (#rgn:region) (#i:id)
             (prf_table: prf_table rgn i)
 	    (aead_entries:Seq.seq (aead_entry i))
 	    (h:mem{safeId i}) : GTot Type0 =
   let open FStar.SeqProperties in
+  (* 1. Each aead entry is refined by the PRF table *)
   (forall (aead_entry:aead_entry i).
     aead_entries `contains` aead_entry ==>
     refines_one_entry prf_table aead_entry h) /\
+  (* 2. Every iv that does not appear in the aead table is unused in the PRF table *)
   (forall (iv:Cipher.iv (alg i)).
     match find_aead_entry iv aead_entries with
     | Some _ -> True //already covered by refines_one_entry
     | None   -> unused_aead_iv_for_prf prf_table iv h)
 
+(** aead_liveness:
+	The aead_state and its regions etc. are live **)
 let aead_liveness (#i:id) (#rw:rw) (st:aead_state i rw) (h:mem) : Type0 =
   HS.(h.h `Map.contains` st.prf.mac_rgn) /\      //contains the mac region
   (safeId i ==> h `HS.contains` st.log) /\       //contains the aead log
   (prf i ==> h `HS.contains` (itable i st.prf)) //contains the prf table
 
-(*** MAIN STATEFUL INVARIANT ***)
+
+(*** inv st h:
+       The final stateful invariant,
+       refines and aead_state_live ***)
 let inv (#i:id) (#rw:rw) (st:aead_state i rw) (h:mem) : Type0 =
   aead_liveness st h /\
   (safeId i ==>
@@ -217,41 +277,46 @@ let inv (#i:id) (#rw:rw) (st:aead_state i rw) (h:mem) : Type0 =
       let aead_entries = HS.sel h st.log in
       refines prf_table aead_entries h))
 
-(* TODO: Move this out of here to be closer to AEAD.encrypt, where it is mainly used *)
-let modifies_table_above_x_and_buffer (#i:id) (#l:nat) (t:PRF.state i)
-				      (x:PRF.domain i) (b:lbuffer l)
-				      (h0:HS.mem) (h1:HS.mem) =
-  Buffer.live h1 b /\
-  (if prf i then
-    let r = PRF.itable i t in
-    let rb = Buffer.frameOf b in
-    let rgns = Set.union (Set.singleton #HH.rid t.rgn) (Set.singleton #HH.rid rb) in
-    let contents0 = HS.sel h0 r in
-    let contents1 = HS.sel h1 r in
-    HS.modifies rgns h0 h1 /\
-    HS.modifies_ref t.rgn (TSet.singleton (FStar.Heap.Ref (HS.as_ref r))) h0 h1 /\
-    Buffer.modifies_buf_1 rb b h0 h1 /\
-    Seq.length contents0 <= Seq.length contents1 /\
-    Seq.equal (Seq.slice contents1 0 (Seq.length contents0)) contents0 /\
-    all_above (Seq.slice contents1 (Seq.length contents0) (Seq.length contents1)) x
-  else
-    Buffer.modifies_1 b h0 h1)
 
-(* The ctr value associated with the first otp block *)
-let otp_offset (i:id) = ctr_0 i +^ 1ul
+(*** SEPARATION AND LIVENESS
+     REQUIREMENTS OF THE INTERFACE ***)
 
-let remaining_len_ok (#i:id) (current_block_index:PRF.domain i) (len:u32) (remaining_len:u32) =
-  PRF.ctr_0 i <^ current_block_index.ctr &&
-  safelen i (v remaining_len) current_block_index.ctr &&
-  remaining_len <=^ len &&
-  len <> 0ul &&
-  safelen i (v len) (otp_offset i) &&
-  (let completed_len = v len - v remaining_len in
-   let n_blocks = v current_block_index.ctr - v (otp_offset i) in
-   if remaining_len = 0ul then
-      n_blocks = num_blocks_for_len i (v len)
-   else completed_len = FStar.Mul.(n_blocks * v (PRF.blocklen i)))
+module Plain = Crypto.Plain
+(** enc_dec_separation:
+	Calling AEAD.encrypt/decrypt requires this separation **)
+let enc_dec_separation (#i:id) (#rw:rw) (st:aead_state i rw)
+		       (#aadlen:nat) (aad: lbuffer aadlen)
+		       (#plainlen:nat) (plain: plainBuffer i plainlen)
+		       (#cipherlen: nat) (cipher:lbuffer cipherlen) =
+    Buffer.disjoint aad cipher /\
+    Buffer.disjoint (Plain.as_buffer plain) aad /\
+    Buffer.disjoint (Plain.as_buffer plain) cipher /\
+    HS.is_eternal_region st.log_region /\
+    HS.is_eternal_region (Buffer.frameOf cipher) /\ // why?
+    HS.is_eternal_region (Buffer.frameOf (Plain.as_buffer plain)) /\ //why?
+    HS.is_eternal_region (Buffer.frameOf aad) /\ //why?
+    HH.disjoint (Buffer.frameOf (Plain.as_buffer plain)) st.log_region /\
+    HH.disjoint (Buffer.frameOf cipher) st.log_region /\
+    HH.disjoint (Buffer.frameOf aad) st.log_region /\
+    st.log_region <> HH.root /\
+    Buffer.frameOf cipher <> HH.root /\
+    Buffer.frameOf aad <> HH.root /\
+    Buffer.frameOf (Plain.as_buffer plain) <> HH.root
 
+(** enc_dec_liveness:
+	Calling AEAD.encrypt/decrypt requires and ensures this liveness **)
+let enc_dec_liveness (#i:id) (#rw:rw) (st:aead_state i rw)
+		  (#aadlen:nat) (aad: lbuffer aadlen)
+		  (#plainlen:nat) (plain: plainBuffer i plainlen)
+		  (#cipherlen: nat) (cipher:lbuffer cipherlen) (h:mem) =
+    let open HS in
+    Buffer.live h aad /\
+    Buffer.live h cipher /\
+    Plain.live h plain /\
+    st.log_region `is_in` h.h
+
+(*** SOME BASIC LEMMAS USED 
+     THROUGHOUT Crypto.AEAD.* ***)
 let incr_remaining_len_ok (#i:id) (x:PRF.domain i) (len:u32) (remaining_len:u32)
     : Lemma (let l = min remaining_len (PRF.blocklen i) in
 	     remaining_len_ok x len remaining_len /\
@@ -263,3 +328,72 @@ let init_remaining_len_ok (#i:id) (x:PRF.domain i{PRF.ctr_0 i +^ 1ul = x.ctr})
 			  (len:u32{len <> 0ul /\ safelen i (v len) x.ctr})
     : Lemma (remaining_len_ok x len len)
     = ()
+
+let u (n:FStar.UInt.uint_t 32) = uint_to_t n
+
+(** Framing lemmas for clauses of the main invariant **)
+#reset-options "--initial_fuel 0 --max_fuel 0 --initial_ifuel 0 --max_ifuel 0"
+let frame_refines_one_entry (#i:id{safeId i}) (#mac_rgn:region) 
+			    (h:mem) (h':mem) 
+			    (blocks:prf_table mac_rgn i)
+			    (e:aead_entry i) 
+   : Lemma (requires (let open HS in
+		      refines_one_entry blocks e h /\			    
+		      HH.modifies_rref mac_rgn TSet.empty h.h h'.h /\
+		      live_region h' mac_rgn))
+	   (ensures  refines_one_entry blocks e h')
+   = ()
+
+let frame_unused_aead_iv_for_prf (#mac_rgn:region) (#i:id) (h0:mem{safeId i}) (h1:mem)
+				 (prf_table:prf_table mac_rgn i)
+				 (iv:Cipher.iv (alg i))
+  : Lemma (requires (let open HS in
+		     unused_aead_iv_for_prf prf_table iv h0        /\
+                     HH.modifies_rref mac_rgn TSet.empty h0.h h1.h /\
+		     live_region h1 mac_rgn))
+	  (ensures  unused_aead_iv_for_prf prf_table iv h1)
+  = ()
+
+let frame_refines (i:id{safeId i}) (mac_rgn:region) 
+		  (blocks:prf_table mac_rgn i)
+		  (entries:aead_entries i)
+		  (h:mem) (h':mem)
+   : Lemma (requires (let open HS in 
+		      refines blocks entries h                     /\
+   		      HH.modifies_rref mac_rgn TSet.empty h.h h'.h /\
+		      HS.live_region h' mac_rgn))
+	   (ensures  refines blocks entries h')
+   = let open FStar.Classical in
+     forall_intro (move_requires (frame_refines_one_entry h h' blocks));
+     forall_intro (move_requires (frame_unused_aead_iv_for_prf h h' blocks))
+
+let weaken_all_above (#rgn:region) (#i:id) (s:Seq.seq (PRF.entry rgn i)) 
+		    (x:PRF.domain i) (y:PRF.domain i{y `above` x})
+    : Lemma (all_above y s ==> all_above x s)
+    = ()
+
+(** counterblocks_emp:
+	proves that counterblocks on a zero range is the empty sequence
+ **)
+#set-options "--initial_fuel 1 --max_fuel 1 --initial_ifuel 0 --max_ifuel 0"
+let counterblocks_emp   (i:id)
+			(rgn:region)
+			(x:PRF.domain i{ctr_0 i <^ PRF.(x.ctr) })
+			(l:nat)
+			(to_pos:nat{to_pos <= l /\ safelen i 0 PRF.(x.ctr)})
+			(plain:Plain.plain i l)
+			(cipher:lbytes l)
+   : Lemma (safeId i ==> counterblocks i rgn x l to_pos to_pos plain cipher == Seq.createEmpty)
+   = ()
+
+(** Lemmas about searching for entries in prf_blocks **)
+let find_append (#i:id) (#r:rid) (d:domain i) (s1:prf_table r i) (s2:prf_table r i)
+   : Lemma (requires (None? (find s1 d)))
+           (ensures (find (Seq.append s1 s2) d == find s2 d))
+   = SeqProperties.find_append_none s1 s2 (is_entry_domain d)
+
+#set-options "--initial_ifuel 0 --max_ifuel 0 --initial_fuel 2 --max_fuel 2"
+let find_singleton (#rgn:region) (#i:id) (e:PRF.entry rgn i) (x:PRF.domain i) 
+    : Lemma (if is_entry_domain x e then PRF.find (Seq.create 1 e) x == Some e.range
+	     else PRF.find (Seq.create 1 e) x == None)
+    = ()	     
